added exporter keys to Epochs state and to the QUIC API; extended TestQUIC to reconnect with tickets

src/tls/test/mitls.ml
@@ -94,7 +94,9 @@ let setalpn x =
   config := {!config with alpn = Some al}
 
 let setquic () =
+  quic := true;
   config := {!config with
+    non_blocking_read = true;
     quic_parameters = Some ([QuicVersion1],[
       Quic_initial_max_stream_data(65536);
       Quic_initial_max_data(16777216);
@@ -132,7 +134,7 @@ let offer_psk x =
   let ids = BatString.nsplit x ":" in
   let add_psk y =
     if List.mem y !loaded_psk then
-      offered_psk := (Platform.Bytes.utf8 y) :: !offered_psk
+      offered_psk := Platform.Bytes.utf8 y :: !offered_psk
     else
       failwith ("Cannot offer PSK with label "^y^" without loading it first")
     in
@@ -158,12 +160,11 @@ let _ =
     ("-tlsapi", Arg.Unit (fun () -> ()), "run through the TLS API (legacy, always on)");
     ("-verify", Arg.Unit (fun () -> config := {!config with check_peer_certificate = true;}), "enforce peer certificate validation");
     ("-ffi", Arg.Unit (fun () -> ffi := true), "test FFI instead of API");
-    ("-quic", Arg.Unit (fun () -> quic := true), "test QUIC API");
     ("-noems", Arg.Unit (fun () -> config := {!config with extended_master_secret = false;}), "disable extended master secret support");
     ("-ciphers", Arg.String setcs, "colon-separated list of cipher suites; see above for valid values");
     ("-sigalgs", Arg.String setsa, "colon-separated list of signature algorithms; see above for valid values");
     ("-alpn", Arg.String setalpn, "colon-separated list of application-level protocols");
-    ("-quic", Arg.Unit setquic, "handle the QuicTransportParameters extension");
+    ("-quic", Arg.Unit setquic, "test QUIC API, using the QuicTransportParameters extension");
     ("-reconnect", Arg.Unit (fun () -> reconnect := true), "reconnect at the end of the session, using received ticket (client only)");
     ("-groups", Arg.String setng, "colon-separated list of supported named groups; see above for valid values");
     ("-shares", Arg.String setog, "colon-separated list of named groups to offer shares on, as a TLS 1.3 client");
@@ -184,19 +185,30 @@ let _ =
     in
 
   match !role with
-  | Client when !ffi -> TestFFI.client !config host (Z.of_int port)
-  | Server when !ffi -> TestFFI.server !config host (Z.of_int port)
-  | Client when !quic -> TestQUIC.client !config host (Z.of_int port)
-  | Server when !quic -> TestQUIC.server !config host (Z.of_int port)
   | Client ->
-    (let _ = TestAPI.client !config host (Z.of_int port) None (!offered_psk) in
-    match !reconnect, !config.peer_name with
-    | true, Some h ->
-      let (opsk, ot12) =
-        match Ticket.lookup h with
-        | None -> !offered_psk, None
-        | Some (t, true) -> t :: !offered_psk, None
-        | Some (t, false) -> !offered_psk, Some t in
-      TestAPI.client !config host (Z.of_int port) ot12 opsk
-    | _ -> ())
-  | Server -> TestAPI.server !config host (Z.of_int port)
+     if !ffi then
+       TestFFI.client !config host (Z.of_int port)
+     else (
+       ( if !quic then
+           TestQUIC.client !config host (Z.of_int port) !offered_psk
+         else 
+           TestAPI.client !config host (Z.of_int port) None !offered_psk);
+       match !reconnect, !config.peer_name with
+       | true, Some h ->
+          let (opsk, ot12) =
+            match Ticket.lookup h with
+            | None -> !offered_psk, None
+            | Some (t, true) -> t :: !offered_psk, None
+            | Some (t, false) -> !offered_psk, Some t in
+          if !quic then
+            TestQUIC.client !config host (Z.of_int port) opsk
+          else
+            TestAPI.client !config host (Z.of_int port) ot12 opsk 
+       | _ -> ())
+  | Server ->
+     if !quic then
+       TestQUIC.server !config host (Z.of_int port)
+     else if !ffi then
+       TestFFI.server !config host (Z.of_int port)
+     else
+       TestAPI.server !config host (Z.of_int port)
